add headers to files

theories/logrel/subtyping.v
@@ -1,4 +1,10 @@
-From actris.logrel Require Export model.
+(** This file contains the definition of the semantic subtyping relation
+[A <: B], where [A] and [B] can be either term types or session types, as
+well as a semantic type equivalence relation [A <:> B], which is essentially
+equivalent to having both [A <: B] and [B <: A]. Finally, the notion of a
+*copyable type* is defined in terms of subtyping: a type [A] is copyable
+when [A <: copy A]. *)
+From actris.logrel Require Export model term_types.
 
 Definition lty_le {Σ k} : lty Σ k → lty Σ k → iProp Σ :=
   match k with
@@ -14,6 +20,10 @@ Definition lty_bi_le {Σ k} (M1 M2 : lty Σ k) : iProp Σ :=
 Arguments lty_bi_le : simpl never.
 Infix "<:>" := lty_bi_le (at level 70) : bi_scope.
 Instance: Params (@lty_bi_le) 2 := {}.
+
+Definition lty_copyable {Σ} (A : ltty Σ) : iProp Σ :=
+  tc_opaque (A <: lty_copy A)%I.
+Instance: Params (@lty_copyable) 1 := {}.
 
 Section subtyping.
   Context {Σ : gFunctors}.
@@ -31,4 +41,9 @@ Section subtyping.
   Proof. solve_proper. Qed.
   Global Instance lty_bi_le_proper {k} : Proper ((≡) ==> (≡) ==> (≡)) (@lty_bi_le Σ k).
   Proof. solve_proper. Qed.
+
+  Global Instance lty_copyable_plain A : Plain (@lty_copyable Σ A).
+  Proof. rewrite /lty_copyable /=. apply _. Qed.
+  Global Instance lty_copyable_ne : NonExpansive (@lty_copyable Σ).
+  Proof. rewrite /lty_copyable /=. solve_proper. Qed.
 End subtyping.
